src/TwoDisk/TwoDiskTheorems.v
@@ -53,7 +53,7 @@ Hint Resolve holds_in_none_eq.
 Hint Resolve pred_missing.
 
 Theorem TDRead0_ok : forall (i: Interface TD.API) a,
-    prog_rok
+    prog_ok
       (fun '(d_0, F) state =>
          {|
            pre := TD.disk0 state |= eq d_0 /\
@@ -83,7 +83,7 @@ Proof.
 Qed.
 
 Theorem TDRead1_ok : forall (i: Interface TD.API) a,
-    prog_rok
+    prog_ok
       (fun '(F, d_1) state =>
          {|
            pre := TD.disk0 state |= F /\
@@ -113,7 +113,7 @@ Proof.
 Qed.
 
 Theorem TDWrite0_ok : forall (i: Interface TD.API) a b,
-    prog_rok
+    prog_ok
       (fun '(d_0, F) state =>
          {|
            pre := TD.disk0 state |= eq d_0 /\
@@ -148,7 +148,7 @@ Proof.
 Qed.
 
 Theorem TDWrite1_ok : forall (i: Interface TD.API) a b,
-    prog_rok
+    prog_ok
       (fun '(F, d_1) state =>
          {|
            pre := TD.disk0 state |= F /\
@@ -183,7 +183,7 @@ Proof.
 Qed.
 
 Theorem TDDiskSize0_ok : forall (i: Interface TD.API),
-    prog_rok
+    prog_ok
       (fun '(d_0, F) state =>
          {|
            pre := TD.disk0 state |= eq d_0 /\
@@ -214,7 +214,7 @@ Proof.
 Qed.
 
 Theorem TDDiskSize1_ok : forall (i: Interface TD.API),
-    prog_rok
+    prog_ok
       (fun '(F, d_1) state =>
          {|
            pre := TD.disk0 state |= F /\
